Regex/Interval/Intersection.lean
@@ -4,129 +4,128 @@ import Regex.Interval.Basic
 import Regex.Interval.Lemmas
 
 /-!
-## IntervalSet
+## Interval Set
 
-IntervalSet operations like `Interval.intersection`
+IntervalSet operations like `IntervalSet.canonicalize` or `IntervalSet.intersection`
 -/
 
-namespace Interval
+namespace IntervalSet
 
-def Acc.with_none (acc : Acc) (n : Range Char) (h : acc.next.isNone) : Acc :=
-  {acc with next := n, nonOverlapping := nonOverlappingWithLast_of_none acc n h}
+def Acc.with_none (acc : Interval.Acc) (n : NonemptyInterval Char) (h : acc.next.isNone)
+    : Interval.Acc :=
+  {acc with next := n, nonOverlapping := Intervals.nonOverlappingWithLast_of_none acc n h}
 
-def Acc.with_next (acc : Acc) (n : Range Char) (h1 : is_start_eq acc.next n) : Acc :=
-  {acc with next := n, nonOverlapping := nonOverlappingWithLast_of_val acc n h1}
+def Acc.with_next (acc : Interval.Acc) (n : NonemptyInterval Char)
+  (h1 : Interval.is_start_eq acc.next n) : Interval.Acc :=
+  {acc with next := n, nonOverlapping := Intervals.nonOverlappingWithLast_of_val acc n h1}
 
-def Acc.with_next_set (acc : Acc) (l r : Range Char) (h1 : Range.nonOverlapping l r)
-  (h2 : acc.next = some l) : Acc :=
-  match hm : acc.set.ranges.last? with
+def Acc.with_next_set (acc : Interval.Acc) (l r : NonemptyInterval Char)
+  (h1 : Interval.nonOverlapping l r) (h2 : acc.next = some l) : Interval.Acc :=
+  match hm : acc.set.intervals.last? with
   | some _ =>
-    have : Ranges.nonOverlapping (Array.push acc.set.ranges l) :=
-              nonOverlapping_of_push acc l hm h2
+    have : Intervals.nonOverlapping (Array.push acc.set.intervals l) :=
+              Intervals.nonOverlapping_of_push acc l hm h2
     {acc with next := r,
-              set := Acc.push acc l this,
-              nonOverlapping := nonOverlappingWithLast_of_push acc h2 this h1}
+              set := Interval.Acc.push acc l this,
+              nonOverlapping := Intervals.nonOverlappingWithLast_of_push acc h2 this h1}
   | none =>
-    {acc with next := r, set := Interval.singleton l,
-              nonOverlapping := nonOverlappingWithLast_of_singleton l r h1}
+    {acc with next := r, set := Intervals.singleton l,
+              nonOverlapping := Intervals.nonOverlappingWithLast_of_singleton l r h1}
 
-instance : Inhabited Acc :=
-  ⟨⟨none, default, nonOverlappingWithLast_of_empty default none
+instance : Inhabited Interval.Acc :=
+  ⟨⟨none, default, Intervals.nonOverlappingWithLast_of_empty default none
                         (Array.default_size_zero default (by simp))⟩⟩
 
 /-- Converts `ranges` into `IntervalSet` with canonical ordering.  -/
-def canonicalize (ranges : Array (Range Char)) : IntervalSet Char :=
+def canonicalize (ranges : Array (NonemptyInterval Char)) : IntervalSet Char :=
   let _ranges := Array.qsort ranges
-                  (fun a b => a.start = b.start && a.end < b.end || a.start < b.start)
-  let _ranges := Ranges.unique _ranges
+                  (fun a b => a.fst = b.fst && a.snd < b.snd || a.fst < b.fst)
+  let _ranges := Intervals.unique _ranges
 
-  let init : Acc := default
+  let init : Interval.Acc := default
   let acc := _ranges |> Array.foldl (init := init) (fun acc r =>
     match hm : acc.next with
     | some l =>
-      if h1 : (r.start.toNat - l.end.toNat) = 1 then  -- [a-bc-d] => [a-d]
-        let next : Range Char := ⟨l.start, r.end, by
-            have hx : l.end < r.start := by simp [Char.succ_lt h1]
-            have hy : l.end ≤ r.start := by simp [Char.lt_le hx]
-            have hz : l.start ≤ r.start := by simp [Char.le_trans l.isLe hy]
-            simp [Char.le_trans hz r.isLe]
+      if h1 : (r.fst.toNat - l.snd.toNat) = 1 then  -- [a-bc-d] => [a-d]
+        let next : NonemptyInterval Char := ⟨⟨l.fst, r.snd⟩, by
+            have hx : l.snd < r.fst := by simp [Char.succ_lt h1]
+            have hy : l.snd ≤ r.fst := by simp [Char.lt_le hx]
+            have hz : l.fst ≤ r.fst := by simp [Char.le_trans l.fst_le_snd hy]
+            simp [Char.le_trans hz r.fst_le_snd]
         ⟩
-        Acc.with_next acc next (is_start_eq_of_val acc.next next hm (by simp))
-      else if h2 : l.start = r.start then -- [a-ca-d] => [a-d]
-        if l.end < r.end
+        Acc.with_next acc next (Intervals.is_start_eq_of_val acc.next next hm (by simp))
+      else if h2 : l.fst = r.fst then -- [a-ca-d] => [a-d]
+        if l.snd < r.snd
         then
-          let next : Range Char := ⟨l.start, r.end, by
-            have hx : l.start ≤ r.start := by simp [Char.eq_le h2]
-            simp [Char.le_trans hx r.isLe]
+          let next : NonemptyInterval Char := ⟨⟨l.fst, r.snd⟩, by
+            have hx : l.fst ≤ r.fst := by simp [Char.eq_le h2]
+            simp [Char.le_trans hx r.fst_le_snd]
           ⟩
-          Acc.with_next acc next (is_start_eq_of_val acc.next next hm (by simp))
-        else acc -- r.start = l.start ∧ r.end < l.end
-      else if h2 : r.start < l.end then -- [a-cb-d] => [a-d]
-        if r.end ≤ l.end -- [a-eb-d] => [a-e]
+          Acc.with_next acc next (Intervals.is_start_eq_of_val acc.next next hm (by simp))
+        else acc -- r.fst = l.fst ∧ r.snd < l.snd
+      else if h2 : r.fst < l.snd then -- [a-cb-d] => [a-d]
+        if r.snd ≤ l.snd -- [a-eb-d] => [a-e]
         then acc
-        else if h : l.start < r.start -- [a-cb-d] => [a-d]
+        else if h : l.fst < r.fst -- [a-cb-d] => [a-d]
         then
-          let next : Range Char := ⟨l.start, r.end, by
-            have hx : l.start ≤ r.start := by simp [Char.lt_le h]
-            simp [Char.le_trans hx r.isLe]
+          let next : NonemptyInterval Char := ⟨⟨l.fst, r.snd⟩, by
+            have hx : l.fst ≤ r.fst := by simp [Char.lt_le h]
+            simp [Char.le_trans hx r.fst_le_snd]
           ⟩
-          Acc.with_next acc next (is_start_eq_of_val acc.next next hm (by simp))
-        else -- ¬l.start = r.start ∧ ¬l.start < r.start => r.start < l.start
+          Acc.with_next acc next (Intervals.is_start_eq_of_val acc.next next hm (by simp))
+        else -- ¬l.fst = r.fst ∧ ¬l.fst < r.fst => r.fst < l.fst
           panic s!"internal error: array not sorted at {l} {r}"
-      else if l.end = r.start && r.start = r.end then acc
-      else if h3 : l.end = r.start then -- [a-bb-c] => [a-c]
-        let next : Range Char := ⟨l.start, r.end, by
-          have hx : l.end ≤ r.start := by simp [Char.eq_le h3]
-          have hy : l.start ≤ r.start := by simp [Char.le_trans l.isLe hx]
-          simp [Char.le_trans hy r.isLe]
+      else if l.snd = r.fst && r.fst = r.snd then acc
+      else if h3 : l.snd = r.fst then -- [a-bb-c] => [a-c]
+        let next : NonemptyInterval Char := ⟨⟨l.fst, r.snd⟩, by
+          have hx : l.snd ≤ r.fst := by simp [Char.eq_le h3]
+          have hy : l.fst ≤ r.fst := by simp [Char.le_trans l.fst_le_snd hx]
+          simp [Char.le_trans hy r.fst_le_snd]
         ⟩
-        Acc.with_next acc next (is_start_eq_of_val acc.next next hm (by simp))
-      else if r.start < l.start then panic s!"internal error: array not sorted at {l} {r}"
+        Acc.with_next acc next (Intervals.is_start_eq_of_val acc.next next hm (by simp))
+      else if r.fst < l.fst then panic s!"internal error: array not sorted at {l} {r}"
       else -- [a-eg-h] => [a-eg-h]
-        have : Range.nonOverlapping l r := isNonOverlapping l r h1 h2 h3
+        have : Interval.nonOverlapping l r := Intervals.isNonOverlapping l r h1 h2 h3
         Acc.with_next_set acc l r this hm
     | none => Acc.with_none acc r (by unfold Option.isNone; simp_all [hm]))
 
   let intervalSet :=
     match hm : acc.next with
     | some v =>
-        match hn : acc.set.ranges.last? with
-        | some _ => Acc.push acc v (nonOverlapping_of_push acc v hn (by simp[hm]; simp_all))
-        | none => Interval.singleton v
+        match hn : acc.set.intervals.last? with
+        | some _ => Interval.Acc.push acc v
+            (Intervals.nonOverlapping_of_push acc v hn (by simp[hm]; simp_all))
+        | none => Intervals.singleton v
     | none => acc.set
 
   intervalSet
 
-/-- Negate a interval set wrt the corresponding `Bound` . -/
+/-- Negate a interval set wrt the corresponding BoundedOrder `instBoundedOrderCharInstLEChar` . -/
 def negate (interval : IntervalSet Char) : IntervalSet Char :=
-  if interval.ranges.size = 0
+  if interval.intervals.size = 0
   then
-    singleton ⟨(Bound.min_value : Char), Bound.max_value, Bound.min_value_le_max_value⟩
+    Intervals.singleton ⟨⟨Bot.bot, Top.top⟩, OrderBot.bot_le Top.top⟩
   else
-    let ranges : Array (Range Char) :=
-      Array.mapIdx interval.ranges  (fun i x => (i, x))
+    let ranges : Array (NonemptyInterval Char) :=
+      Array.mapIdx interval.intervals  (fun i x => (i, x))
       |> Array.map (fun (i, y) =>
         if h : 0 < i.val
         then
-          let x := interval.ranges.get ⟨i - 1, Fin.pred h⟩
-          let y := interval.ranges.get i
-          Range.negate x y
-            (Interval.nonOverlapping_of_pred interval.ranges i x y h
+          let x := interval.intervals.get ⟨i - 1, Intervals.Fin.pred h⟩
+          let y := interval.intervals.get i
+          Interval.between x y
+            (Intervals.nonOverlapping_of_pred interval.intervals i x y h
                         (by simp) (by simp) interval.isNonOverlapping)
         else
-          if Bound.min_value < y.start
-          then ⟨Bound.min_value, Bound.decrement y.start, by
-              simp [Bound.min_value_le_decrement y.start]
-            ⟩
+          if Bot.bot < y.fst
+          then ⟨⟨ Bot.bot, Char.decrement y.fst⟩ , by simp⟩
           else y
         )
-    let last : Array (Range Char) :=
-      match interval.ranges.pop? with
+    let last : Array (NonemptyInterval Char) :=
+      match interval.intervals.pop? with
       | some (x, _) =>
-          if x.end < Bound.max_value
-          then #[⟨Bound.increment x.end, Bound.max_value, by
-              simp [Bound.increment_le_max_value x.end]
-            ⟩]
+          if x.snd <Top.top
+          then #[⟨⟨Char.increment x.snd, Top.top⟩, by simp⟩]
           else #[]
       | none => #[]
 
@@ -135,18 +134,18 @@ def negate (interval : IntervalSet Char) : IntervalSet Char :=
 
 /-- Intersection of interval sets -/
 def intersection (interval1 interval2 : IntervalSet Char) : IntervalSet Char :=
-  let ranges := intersection.loop 0 0 interval1.ranges interval2.ranges #[]
+  let ranges := intersection.loop 0 0 interval1.intervals interval2.intervals #[]
   canonicalize ranges
 where
-  loop (a b : Nat) (ra rb acc : Array $ Range Char) : Array $ Range Char :=
+  loop (a b : Nat) (ra rb acc : Array $ NonemptyInterval Char) : Array $ NonemptyInterval Char :=
     if h₁ : a < ra.size then
       if h₂ : b < rb.size then
         let acc :=
-          match Range.intersection (ra.get ⟨a, h₁⟩) (rb.get ⟨b, h₂⟩) with
+          match Interval.intersection (ra.get ⟨a, h₁⟩) (rb.get ⟨b, h₂⟩) with
           | some r => acc.push r
           | none => acc
 
-        if (ra.get ⟨a, h₁⟩).end < (rb.get ⟨b, h₂⟩).end
+        if (ra.get ⟨a, h₁⟩).snd < (rb.get ⟨b, h₂⟩).snd
         then loop (a+1) b ra rb acc
         else loop a (b+1) ra rb acc
       else acc
@@ -159,9 +158,9 @@ def difference (interval1 interval2 : IntervalSet Char) : IntervalSet Char :=
 
 /-- Union of interval sets. -/
 def union (interval1 interval2 : IntervalSet Char) : IntervalSet Char :=
-  if interval1.ranges.size = 0 then interval2
-  else if interval2.ranges.size = 0 then interval1
-  else canonicalize (interval1.ranges ++ interval2.ranges)
+  if interval1.intervals.size = 0 then interval2
+  else if interval2.intervals.size = 0 then interval1
+  else canonicalize (interval1.intervals ++ interval2.intervals)
 
 /-- Compute the symmetric difference (A⊖B = (A∪B)\(A∩B)) of the two sets. -/
 def symmetric_difference (interval1 interval2 : IntervalSet Char) : IntervalSet Char :=
