Regex/Interval/Lemmas.lean
@@ -6,6 +6,8 @@ import Std.Data.Int.Lemmas
 import Std.Data.List.Basic
 import Std.Data.Array.Init.Lemmas
 import Mathlib.Data.List.Chain
+import Mathlib.Order.BoundedOrder
+import Mathlib.Order.Interval
 import Regex.Utils
 import Regex.Data.UInt.Basic
 import Regex.Data.Char.Basic
@@ -14,14 +16,16 @@ import Regex.Data.Array.Basic
 import Regex.Data.Array.Lemmas
 import Regex.Interval.Basic
 
-namespace Ranges
+namespace Intervals
 
-theorem empty_isNonOverlapping {α : Type u} [Ord α] [LT α] [LE α] [Bound α] [HSub α α Nat]
-    : nonOverlapping (#[] : Array (Range α)) := by
+open Interval
+
+theorem empty_isNonOverlapping {α : Type u} [LT α] [LE α] [BoundedOrder α] [HSub α α Nat]
+    : nonOverlapping (#[] : Array (NonemptyInterval α)) := by
   unfold nonOverlapping dataIsNonOverlapping
   split <;> simp_all
 
-theorem single_isNonOverlapping (ranges : Array (Range Char)) (h : ranges.size = 1)
+theorem single_isNonOverlapping (ranges : Array (NonemptyInterval Char)) (h : ranges.size = 1)
     : nonOverlapping ranges  := by
   unfold nonOverlapping dataIsNonOverlapping
   split <;> try simp_all
@@ -31,18 +35,14 @@ theorem single_isNonOverlapping (ranges : Array (Range Char)) (h : ranges.size =
   unfold List.length at h
   split at h <;> try simp_all
 
-end Ranges
-
-instance (α : Type u) [Ord α] [LT α] [LE α] [Bound α] [HSub α α Nat]
+instance (α : Type u) [LT α] [LE α] [BoundedOrder α] [HSub α α Nat]
     [(a b : α) → Decidable (a < b)] [(a b : α) → Decidable (a = b)]
     : Inhabited $ IntervalSet α where
-  default := ⟨#[], Ranges.empty_isNonOverlapping⟩
+  default := ⟨#[], Intervals.empty_isNonOverlapping⟩
 
-namespace Interval
-
-def singleton (r : Range Char) : IntervalSet Char :=
+def singleton (r : NonemptyInterval Char) : IntervalSet Char :=
   let arr := #[r]
-  ⟨arr, by simp [Ranges.single_isNonOverlapping arr (Array.size_one r)]⟩
+  ⟨arr, by simp [Intervals.single_isNonOverlapping arr (Array.size_one r)]⟩
 
 theorem pred_lt' {n m : Nat} (h : m < n) : Nat.pred n < n :=
   Nat.pred_lt (Nat.not_eq_zero_of_lt h)
@@ -52,23 +52,24 @@ theorem Fin.pred {i : Fin n} (h : 0 < i.val) : LT.lt (i.val-1) n := by
   have h2 : i.val < n := i.isLt
   simp [Nat.lt_trans h1 h2]
 
-theorem isNonOverlapping (l r : Range Char)
-  (h1 : ¬(r.start.toNat - l.end.toNat) = 1) (h2 : ¬r.start < l.end) (h3 : ¬l.end = r.start)
-    : Range.nonOverlapping l r := by
-  have h1 : ¬1 = (r.start.toNat - l.end.toNat) := fun h => h1 (h.symm)
-  have h2 : l.end ≤  r.start := Nat.not_lt.mp h2
-  have h3 : ¬l.end.val.val = r.start.val.val := UInt32.val_ne_of_ne (Char.val_ne_of_ne h3)
-  have h : l.end.toNat < r.start.toNat := Nat.lt_of_le_of_ne h2 (Fin.val_ne_of_ne h3)
-  have h : l.end.toNat+1 ≤ r.start.toNat := Nat.succ_le_of_lt h
-  have h : 1 + l.end.toNat ≤ r.start.toNat := by rw [Nat.add_comm]; simp [h]
-  have h : 1 < r.start.toNat - l.end.toNat := Nat.lt_of_le_of_ne (Nat.le_sub_of_add_le h) h1
-  unfold Range.nonOverlapping
-  rw [← Range.Char.sub_def]
-  unfold Range.Char.sub
+theorem isNonOverlapping (l r : NonemptyInterval Char)
+  (h1 : ¬(r.fst.toNat - l.snd.toNat) = 1) (h2 : ¬r.fst < l.snd) (h3 : ¬l.snd = r.fst)
+    : Interval.nonOverlapping l r := by
+  have h1 : ¬1 = (r.fst.toNat - l.snd.toNat) := fun h => h1 (h.symm)
+  have h2 : l.snd ≤  r.fst := Nat.not_lt.mp h2
+  have h3 : ¬l.snd.val.val = r.fst.val.val := UInt32.val_ne_of_ne (Char.val_ne_of_ne h3)
+  have h : l.snd.toNat < r.fst.toNat := Nat.lt_of_le_of_ne h2 (Fin.val_ne_of_ne h3)
+  have h : l.snd.toNat+1 ≤ r.fst.toNat := Nat.succ_le_of_lt h
+  have h : 1 + l.snd.toNat ≤ r.fst.toNat := by rw [Nat.add_comm]; simp [h]
+  have h : 1 < r.fst.toNat - l.snd.toNat := Nat.lt_of_le_of_ne (Nat.le_sub_of_add_le h) h1
+  unfold Interval.nonOverlapping
+  rw [← Interval.Char.sub_def]
+  unfold Interval.Char.sub
   simp [h]
 
-theorem nonOverlappingWithLast_of_empty (ranges : Array $ Range Char) (next : Option (Range Char))
-    (h2 : ranges.size = 0) : nonOverlappingWithLast ranges next  := by
+theorem nonOverlappingWithLast_of_empty (ranges : Array $ NonemptyInterval Char)
+  (next : Option (NonemptyInterval Char)) (h2 : ranges.size = 0)
+    : nonOverlappingWithLast ranges next  := by
   unfold nonOverlappingWithLast
   split <;> try simp_all
   · unfold Array.size List.length at h2
@@ -89,8 +90,8 @@ theorem nonOverlappingWithLast_of_empty (ranges : Array $ Range Char) (next : Op
     split at h <;> try simp_all
 
 theorem nonOverlappingWithLast_with_none_eq_empty (acc : Acc) (h : acc.next.isNone)
-    : acc.set.ranges.size = 0 := by
-  have hx : nonOverlappingWithLast acc.set.ranges acc.next := acc.nonOverlapping
+    : acc.set.intervals.size = 0 := by
+  have hx : nonOverlappingWithLast acc.set.intervals acc.next := acc.nonOverlapping
   unfold nonOverlappingWithLast at hx
   split at hx <;> try simp_all
 
@@ -98,62 +99,62 @@ theorem nonOverlappingWithLast_with_none_eq_empty (acc : Acc) (h : acc.next.isNo
   unfold Array.last? at heq
   split at heq <;> try simp_all
 
-theorem nonOverlappingWithLast_of_none (acc : Acc) (n : Range Char) (h : acc.next.isNone)
-    : nonOverlappingWithLast acc.set.ranges n  := by
-  have hx : acc.set.ranges.size = 0 := nonOverlappingWithLast_with_none_eq_empty acc h
-  simp [nonOverlappingWithLast_of_empty acc.set.ranges n hx]
+theorem nonOverlappingWithLast_of_none (acc : Interval.Acc) (n : NonemptyInterval Char) (h : acc.next.isNone)
+    : nonOverlappingWithLast acc.set.intervals n  := by
+  have hx : acc.set.intervals.size = 0 := nonOverlappingWithLast_with_none_eq_empty acc h
+  simp [nonOverlappingWithLast_of_empty acc.set.intervals n hx]
 
-theorem nonOverlappingWithLast_of_val (acc : Acc) (n : Range Char) (h : is_start_eq acc.next n)
-    : nonOverlappingWithLast acc.set.ranges n  := by
-  have hx : nonOverlappingWithLast acc.set.ranges acc.next := acc.nonOverlapping
+theorem nonOverlappingWithLast_of_val (acc : Acc) (n : NonemptyInterval Char)
+  (h : is_start_eq acc.next n) : nonOverlappingWithLast acc.set.intervals n  := by
+  have hx : nonOverlappingWithLast acc.set.intervals acc.next := acc.nonOverlapping
   unfold nonOverlappingWithLast
   unfold nonOverlappingWithLast at hx
   unfold is_start_eq at h
   simp_all
   split <;> try simp_all
-  unfold Range.nonOverlapping
+  unfold Interval.nonOverlapping
   split at hx <;> try simp_all
-  unfold Range.nonOverlapping at hx
+  unfold Interval.nonOverlapping at hx
   simp_all
 
-theorem is_start_eq_of_val (next : Option (Range Char)) (n: Range Char)
-  (hm : next = some l) (hx : l.start = n.start) : is_start_eq next n := by
+theorem is_start_eq_of_val (next : Option (NonemptyInterval Char)) (n: NonemptyInterval Char)
+  (hm : next = some l) (hx : l.fst = n.fst) : is_start_eq next n := by
   unfold is_start_eq
   simp_all
 
-theorem is_start_eq_of_none (next : Option (Range Char)) (n: Range Char)
+theorem is_start_eq_of_none (next : Option (NonemptyInterval Char)) (n: NonemptyInterval Char)
   (hm : next = none) : is_start_eq next n := by
   unfold is_start_eq
   simp_all
 
-theorem nonOverlappingWithLast_of_singleton (l r : Range Char) (h : Range.nonOverlapping l r)
-    : nonOverlappingWithLast (singleton l).ranges (some r)  := by
+theorem nonOverlappingWithLast_of_singleton (l r : NonemptyInterval Char) (h : Interval.nonOverlapping l r)
+    : nonOverlappingWithLast (singleton l).intervals (some r)  := by
   unfold singleton nonOverlappingWithLast
   split <;> simp_all
-  unfold Range.nonOverlapping
+  unfold Interval.nonOverlapping
   rename_i heq _
   unfold Array.last? at heq
   split at heq <;> simp_all
-  unfold Range.nonOverlapping  at h
+  unfold Interval.nonOverlapping  at h
   rename_i last' _ _ _
   have heq' : List.get #[l].data ⟨0, by simp⟩ = l := List.singleton_val l (by simp)
   simp_all
 
-theorem nonOverlapping_of_push (acc : Acc) (next : Range Char)
-  (h1: Array.last? acc.set.ranges = some last) (h2 : acc.next = some next)
-    : Ranges.nonOverlapping (Array.push acc.set.ranges next) := by
-  unfold Array.push Ranges.nonOverlapping
+theorem nonOverlapping_of_push (acc : Acc) (next : NonemptyInterval Char)
+  (h1: Array.last? acc.set.intervals = some last) (h2 : acc.next = some next)
+    : Intervals.nonOverlapping (Array.push acc.set.intervals next) := by
+  unfold Array.push Intervals.nonOverlapping
   simp
-  have ⟨acc', hp⟩ := Array.pop?_of_last? acc.set.ranges h1
-  have h1 : acc.set.ranges.data = acc'.data ++ [last] := Array.concat_of_pop? hp
-  have h2 : Range.nonOverlapping last next := by
-    have hx : nonOverlappingWithLast acc.set.ranges acc.next := acc.nonOverlapping
+  have ⟨acc', hp⟩ := Array.pop?_of_last? acc.set.intervals h1
+  have h1 : acc.set.intervals.data = acc'.data ++ [last] := Array.concat_of_pop? hp
+  have h2 : Interval.nonOverlapping last next := by
+    have hx : nonOverlappingWithLast acc.set.intervals acc.next := acc.nonOverlapping
     unfold nonOverlappingWithLast at hx
     split at hx <;> simp_all
-  have h5 : Ranges.dataIsNonOverlapping (acc'.data ++ [last] ++ [next]) := by
-    have hn : Ranges.nonOverlapping acc.set.ranges := acc.set.isNonOverlapping
-    unfold Ranges.nonOverlapping at hn
-    unfold Ranges.dataIsNonOverlapping
+  have h5 : Intervals.dataIsNonOverlapping (acc'.data ++ [last] ++ [next]) := by
+    have hn : Intervals.nonOverlapping acc.set.intervals := acc.set.isNonOverlapping
+    unfold Intervals.nonOverlapping at hn
+    unfold Intervals.dataIsNonOverlapping
     split <;> simp_all
     rename_i heq
     cases h : acc'.data
@@ -161,17 +162,17 @@ theorem nonOverlapping_of_push (acc : Acc) (next : Range Char)
       simp_all
       rw [← heq.left, ← heq.right]
       rw [← heq.left] at h2
-      have hx : List.Chain Range.nonOverlapping next [] := by simp_all
+      have hx : List.Chain Interval.nonOverlapping next [] := by simp_all
       simp [List.chain_cons.mpr ⟨h2, hx⟩]
       simp [h2]
     · rw [h] at heq
       rename_i head' tail' _ head tail
       have hh : head = head' := List.head_eq_of_cons_eq heq
       have ht : tail ++ [last] ++ [next] = tail' := by simp_all [List.tail_eq_of_cons_eq heq]
-      have hn : List.Chain Range.nonOverlapping head (tail ++ [last]) := by
-        unfold Ranges.dataIsNonOverlapping at hn
+      have hn : List.Chain Interval.nonOverlapping head (tail ++ [last]) := by
+        unfold Intervals.dataIsNonOverlapping at hn
         simp_all [hn]
-      have hy : List.Chain Range.nonOverlapping head (tail ++ [last]  ++ [next]) := by
+      have hy : List.Chain Interval.nonOverlapping head (tail ++ [last]  ++ [next]) := by
         simp [List.chain_append_cons_cons.mpr]
         simp [h2]
         simp [hn]
@@ -203,11 +204,11 @@ theorem Array.eq_succ_of_tail_nth (arr : Array α) (h1 : i+1 < arr.size)
     : tail.get ⟨i, h3⟩ = arr.get ⟨i+1, h1⟩ :=
   List.eq_succ_of_tail_nth arr.data h1 h2 h3
 
-theorem nonOverlapping_of_nth (ranges : Array $ Range Char) (n : Nat)
+theorem nonOverlapping_of_nth (ranges : Array $ NonemptyInterval Char) (n : Nat)
   (h1 : 0 < n) (h2 : n+1 < Array.size ranges) (h3: ranges.data = head :: tail)
   (h4 : ∀ (i : ℕ) (h : i < List.length tail-1),
-    Range.nonOverlapping (tail.get ⟨i, Nat.lt_of_lt_pred h⟩) (tail.get ⟨i+1, Nat.lt_pred_iff.mp h⟩))
-    : Range.nonOverlapping (ranges.get ⟨n, Nat.lt_of_succ_lt h2⟩) (ranges.get ⟨n+1, h2⟩) := by
+    Interval.nonOverlapping (tail.get ⟨i, Nat.lt_of_lt_pred h⟩) (tail.get ⟨i+1, Nat.lt_pred_iff.mp h⟩))
+    : Interval.nonOverlapping (ranges.get ⟨n, Nat.lt_of_succ_lt h2⟩) (ranges.get ⟨n+1, h2⟩) := by
   have hlt : n < Array.size ranges := Nat.lt_of_succ_lt h2
   have hf : n+1 < ranges.data.length := by unfold Array.size at h2; simp_all [h2]
   have hne : ¬n = 0 := (Nat.ne_of_lt h1).symm
@@ -219,7 +220,7 @@ theorem nonOverlapping_of_nth (ranges : Array $ Range Char) (n : Nat)
   have ht1 : n-1 < tail.length-1 := Nat.pred_lt_pred (by simp_all) ht0
   have ht2 : n-1 < tail.length := Nat.lt_of_lt_pred ht1
   have ht3 : n-1+1 < tail.length := by simp [hps, ht0]
-  have : Range.nonOverlapping (tail.get ⟨n-1, ht2⟩) (tail.get ⟨n-1+1, ht3⟩) := h4 (n-1) ht1
+  have : Interval.nonOverlapping (tail.get ⟨n-1, ht2⟩) (tail.get ⟨n-1+1, ht3⟩) := h4 (n-1) ht1
   have : tail.get ⟨n-1, ht2⟩ = ranges.get ⟨n, hlt⟩ := by
     let i := n-1
     have h : i+1 < ranges.size := by simp [hps, hlt]
@@ -232,13 +233,13 @@ theorem nonOverlapping_of_nth (ranges : Array $ Range Char) (n : Nat)
     simp [hps]
   simp_all
 
-theorem nonOverlapping_of_pred (ranges : Array $ Range Char) (i : Fin (Array.size ranges))
-  (x y : Range Char) (h : 0 < i.val)
+theorem nonOverlapping_of_pred (ranges : Array $ NonemptyInterval Char) (i : Fin (Array.size ranges))
+  (x y : NonemptyInterval Char) (h : 0 < i.val)
   (hx : x = Array.get ranges ⟨i-1, Fin.pred h⟩) (hy : y = Array.get ranges i)
-  (hr : Ranges.nonOverlapping ranges)
-   : Range.nonOverlapping x y := by
-  unfold Ranges.nonOverlapping at hr
-  unfold Ranges.dataIsNonOverlapping at hr
+  (hr : Intervals.nonOverlapping ranges)
+   : Interval.nonOverlapping x y := by
+  unfold Intervals.nonOverlapping at hr
+  unfold Intervals.dataIsNonOverlapping at hr
   split at hr <;> try simp_all
   · rename_i heq
     have : 0 = ranges.size := by unfold Array.size List.length; split <;> try simp_all
@@ -256,33 +257,33 @@ theorem nonOverlapping_of_pred (ranges : Array $ Range Char) (i : Fin (Array.siz
       rename_i xt
       have hx1 : 0 < ranges.size := by simp [Nat.lt_trans h hf]
       have hx2 : 0 < tail.length := by cases tail <;> simp_all
-      have : Range.nonOverlapping head (List.get tail { val := 0, isLt := hx2}) := h1 hx2
+      have : Interval.nonOverlapping head (List.get tail { val := 0, isLt := hx2}) := h1 hx2
       have : head = ranges.get ⟨0, hx1⟩  := Array.eq_head_of_get_first ranges hx1 heq
       have : tail.get ⟨0, hx2⟩  = ranges.get ⟨1, hf⟩ := Array.eq_succ_of_tail_nth ranges hf heq hx2
       simp_all
     | ⟨n+2, hf⟩ =>
       have hx1 : n+1 < ranges.size := by simp [Nat.lt_trans _ hf]
-      have hx2 : Range.nonOverlapping ranges[n+1] ranges[n+2] :=
+      have hx2 : Interval.nonOverlapping ranges[n+1] ranges[n+2] :=
         nonOverlapping_of_nth ranges (n+1) (by simp) hf heq h2
       simp [hx2]
 
 theorem nonOverlappingWithLast_of_push(acc : Acc) (h1 : acc.next = some l)
-  (h2 : Ranges.nonOverlapping (Array.push acc.set.ranges l)) (h3 : Range.nonOverlapping l r)
-    : nonOverlappingWithLast (Acc.push acc l h2).ranges (some r) := by
+  (h2 : Intervals.nonOverlapping (Array.push acc.set.intervals l)) (h3 : Interval.nonOverlapping l r)
+    : nonOverlappingWithLast (Acc.push acc l h2).intervals (some r) := by
   unfold Acc.push Array.push nonOverlappingWithLast
   split <;> try simp_all
   rename_i last next heq _
   unfold Array.last? at heq
   split at heq <;> try simp_all
-  have hne : acc.set.ranges.data ++ [l] ≠ [] := by simp_all
-  have h : List.getLast (acc.set.ranges.data ++ [l]) hne
-      = List.get (acc.set.ranges.data ++ [l]) ⟨acc.set.ranges.data.length, (by simp_all)⟩ := by
-      have h : List.get (acc.set.ranges.data ++ [l]) ⟨acc.set.ranges.data.length, (by simp_all)⟩
-              = List.get (acc.set.ranges.data ++ [l])
-                  ⟨(acc.set.ranges.data ++ [l]).length-1, (by simp_all)⟩ := by
-        simp_all
-      rw [h]
-      rw [List.getLast_eq_get (acc.set.ranges.data ++ [l]) hne]
+  have hne : acc.set.intervals.data ++ [l] ≠ [] := by simp_all
+  have h : List.getLast (acc.set.intervals.data ++ [l]) hne
+    = List.get (acc.set.intervals.data ++ [l]) ⟨acc.set.intervals.data.length, (by simp_all)⟩ := by
+    have h : List.get (acc.set.intervals.data ++ [l]) ⟨acc.set.intervals.data.length, (by simp_all)⟩
+            = List.get (acc.set.intervals.data ++ [l])
+                ⟨(acc.set.intervals.data ++ [l]).length-1, (by simp_all)⟩ := by
+      simp_all
+    rw [h]
+    rw [List.getLast_eq_get (acc.set.intervals.data ++ [l]) hne]
   rw [← h] at heq
   simp [List.getLast_append] at heq
   rw [heq] at h3
